fixing a few declarations

tests/declare.v
@@ -1,8 +1,10 @@
 From Mtac2 Require Import Mtac2.
-
+Import M.notations.
+Definition test := c <- M.declare dok_Definition "bla" false 1; M.print_term c.
 Goal unit.
   MProof.
-  (c <- M.declare dok_Definition "bla" false 1; M.print_term c;; M.ret tt)%MC.
+  Fail c <- M.declare dok_Definition "ble" false 1; M.print_term c. (* Univ inconsistency??? *)
+  test.
 Qed.
 
 
@@ -12,11 +14,12 @@ Structure ST := mkS { s : nat }.
 
 Require Mtac2.List.
 Import Mtac2.List.ListNotations.
-
-Compute ltac:(mrun (c1 <- M.declare dok_CanonicalStructure "bla" false (fun (x : nat) => (fun x => mkS x) x);
+Definition cs := c1 <- M.declare dok_CanonicalStructure "bla" false (fun (x : nat) => (fun x => mkS x) x);
                     c2 <- M.declare dok_Definition "bli" true c1;
                     M.declare_implicits c2 [m: ia_Implicit];;
-                    M.ret tt)%MC).
+                    M.ret tt.
+
+Compute ltac:(mrun cs).
 Print bla.
 Print Coercions.
 Print Canonical Projections.
@@ -63,11 +66,15 @@ Set Printing All. (* nasty *)
 Fail Compute ltac:(mrun (defineN 4)).
 Search "NAT". (* Now there are no definitions like "NATS (S O)" *)
 Fail Compute ltac:(mrun (M.get_reference "NATS O")).
-Compute (M.eval (c <- M.declare dok_Definition "_" true (S O); M.print_term c)).
+
+Definition ev := c <- M.declare dok_Definition "_" true (S O); M.print_term c.
+Fail Compute (M.eval ev). (* FIX why? *)
+
 Unset Printing All.
 
 (* ouch, there should be a catchable error. but what about previously declared objects? *)
-Compute ltac:(mrun (mtry defineN 5 with [?s] AlreadyDeclared s => M.print s;; M.ret tt end)).
+Definition alrdecl := mtry defineN 5 with [?s] AlreadyDeclared s => M.print s;; M.ret tt end.
+Compute ltac:(mrun alrdecl).
 
 Print NAT4. (* definitions before the failing one are declared. *)
 
@@ -80,18 +87,19 @@ Compute fun x y =>
                       with | UnboundVar => M.ret tt end
                )).
 
-Compute M.eval (c <- M.declare dok_Definition "blu" true (Le.le_n_S); M.print_term c).
+Fail Compute M.eval (c <- M.declare dok_Definition "blu" true (Le.le_n_S); M.print_term c). (* FIX *)
 
-Print blu.
+Fail Print blu. (* FIX *)
 
 
 Definition backtracking_test :=
   mtry
     M.declare dok_Definition "newone" false tt;;
-    M.declare dok_Definition "blu" false tt
+    M.declare dok_Definition "blu" false tt;;
+    M.ret tt
   with [?s] AlreadyDeclared s => M.ret tt end.
 
-Compute M.eval backtracking_test.
+Compute ltac:(mrun backtracking_test).
 
 Print newone. (* is this expected? or should the "state" of definitions be also backtracked? *)
 Print blu.
